more proof in the example

compcertox/Example.v
@@ -5,7 +5,7 @@ From compcert Require Import
      Clight Ctypes
      LanguageInterface
      Events Globalenvs
-     Smallstep.
+     Smallstep CategoricalComp.
 From compcertox Require Import
   Lifting Encapsulation
   ClightP ClightPComp.
@@ -120,13 +120,13 @@ Section CLIGHTP.
       (Ssequence
          (Ssequence
             (Sset rb_inc1_tmp (Epvar cnt1_id tint))
-            (Sassign
+            (Supdate
                (Epvar cnt1_id tint)
                (Ebinop Cop.Oadd
                        (Epvar cnt1_id tint)
                        (Econst_int (Int.repr 1) tint)
                        tint)))
-         (Sassign
+         (Supdate
             (Epvar cnt1_id tint)
             (Ebinop Cop.Omod
                     (Epvar cnt1_id tint)
@@ -158,13 +158,13 @@ Section CLIGHTP.
       (Ssequence
          (Ssequence
             (Sset rb_inc2_tmp (Epvar cnt2_id tint))
-            (Sassign
+            (Supdate
                (Epvar cnt2_id tint)
                (Ebinop Cop.Oadd
                        (Epvar cnt2_id tint)
                        (Econst_int (Int.repr 1) tint)
                        tint)))
-         (Sassign
+         (Supdate
             (Epvar cnt2_id tint)
             (Ebinop Cop.Omod
                     (Epvar cnt2_id tint)
@@ -372,21 +372,367 @@ End RB_LTS.
 
 Definition rb_spec: semantics li_c (li_c@rb_state) :=
   {|
-    skel := AST.erase_program rb_program;
+    skel := clightp_erase_program rb_program;
     activate se := rb_lts (ClightP.globalenv se rb_program);
     footprint := AST.footprint_of_program rb_program;
   |}.
 
-Instance rb_state_pset : PSet rb_state. Admitted.
+Instance rb_state_pset : PSet rb_state :=
+  {
+    pset_init _ := (fun _ => Vint (Int.zero), 0, 0)%nat;
+  }.
 
 Program Definition rb_espec : li_c +-> li_c :=
-  comp_esem'
-    (encap_prim rb_state)
-    (semantics_embed rb_spec)
-    (skel rb_spec).
+  comp_esem' (encap_prim rb_state) (semantics_embed rb_spec) (skel rb_spec).
 
-Lemma rb_correct: E.forward_simulation (&1) (&1) rb_espec (eclightp rb_program).
+Inductive nat_rel: nat -> Values.val -> Prop :=
+| nat_rel_intro n i
+  (HI: Z.of_nat n = Integers.Int.intval i):
+  nat_rel n (Vint i).
+
+Inductive rb_penv_rel: rb_state -> penv -> Prop :=
+| rb_penv_intro f c1 c2 pe vf vc1 vc2
+  (HA: pe ! arr_id = Some (Array Nz vf (tarray tint Nz)))
+  (HC1: pe ! cnt1_id = Some (Val vc1 tint))
+  (HC2: pe ! cnt2_id = Some (Val vc2 tint))
+  (RA: (forall i, (i < N)%nat -> exists v, ZMap.get (Z.of_nat i) vf = Val v tint /\ v = f i))
+  (RC1: nat_rel c1 vc1) (NC1: (c1 < N)%nat)
+  (RC2: nat_rel c2 vc2) (NC2: (c2 < N)%nat):
+  rb_penv_rel (f, c1, c2) pe.
+
+Inductive rb_query: c_query * rb_state -> c_query * penv -> Prop :=
+| rb_query_intro vf sg vargs m rbst pe
+    (HFLAG: Mem.alloc_flag m = true)
+    (HPE: rb_penv_rel rbst pe):
+  rb_query (cq vf sg vargs m, rbst) (cq vf sg vargs m, pe).
+
+Inductive rb_reply: c_reply * rb_state -> c_reply * penv -> Prop :=
+| rb_reply_intro rv m rbst pe
+    (HFLAG: Mem.alloc_flag m = true)
+    (HPE: rb_penv_rel rbst pe):
+  rb_reply (cr rv m, rbst) (cr rv m, pe).
+
+Program Definition rb_cc: callconv (li_c@rb_state) (li_c@penv) :=
+  {|
+    ccworld := unit;
+    match_senv _ se1 se2 := se1 = se2;
+    match_query _ := rb_query;
+    match_reply _ := rb_reply;
+  |}.
+Next Obligation. reflexivity. Qed.
+Next Obligation. inv H0. reflexivity. Qed.
+Next Obligation. inv H. reflexivity. Qed.
+
+Lemma rb_correct1:
+  E.forward_simulation (&rb_cc) (&1)
+    (encap_prim rb_state)
+    (@encap_prim penv (penv_pset (ClightPComp.vars_of_program rb_program))).
+Proof.
 Admitted.
+
+Inductive rb_func_rel: rb_sig -> function -> Prop :=
+| rb_inc1_rel: rb_func_rel inc1 rb_inc1
+| rb_inc2_rel: rb_func_rel inc2 rb_inc2
+| rb_set_rel: rb_func_rel seti rb_set
+| rb_get_rel: rb_func_rel geti rb_get.
+
+Inductive rb_ms se: rb_internal_state -> state * penv -> Prop :=
+| rb_ms_init:
+  forall vf pe m rbst vs sg func
+    (HFLAG: Mem.alloc_flag m = true)
+    (HPE: rb_penv_rel rbst pe)
+    (HFUN: rb_func_rel sg func)
+    (HF: Genv.find_funct (Genv.globalenv se rb_program) vf
+         = Some (Internal func)),
+    rb_ms se (rb_init sg rbst vs m) (Callstate vf vs Kstop m, pe)
+| rb_ms_final:
+  forall rv pe m rbst
+    (HFLAG: Mem.alloc_flag m = true)
+    (HPE: rb_penv_rel rbst pe),
+    rb_ms se (rb_final rbst rv m) (Returnstate rv Kstop m, pe).
+
+Lemma genv_funct_symbol se id b f (p: ClightP.program):
+  Genv.find_symbol se id = Some b ->
+  (prog_defmap p) ! id = Some (Gfun f) ->
+  Genv.find_funct (ClightP.globalenv se p) (Vptr b Ptrofs.zero) = Some f.
+Proof.
+  intros H1 H2.
+  unfold Genv.find_funct, Genv.find_funct_ptr.
+  destruct Ptrofs.eq_dec; try congruence.
+  apply Genv.find_invert_symbol in H1. cbn.
+  rewrite Genv.find_def_spec. rewrite H1.
+  rewrite H2. reflexivity.
+Qed.
+
+Ltac crush_eval_expr :=
+  cbn;
+  lazymatch goal with
+  | [ |- eval_expr _ _ _ _ _ (Etempvar _ _) _ ] => apply eval_Etempvar; reflexivity
+  | [ |- eval_expr _ _ _ _ _ (Econst_int _ _) _ ] => apply eval_Econst_int
+  | [ |- eval_expr _ _ _ _ _ (Ebinop _ _ _ _) _ ] => eapply eval_Ebinop
+  | [ |- eval_expr _ _ _ _ _ (Evar _ _) _ ] => eapply eval_Elvalue
+  | [ |- eval_expr _ _ _ _ _ (Ederef _ _) _ ] => eapply eval_Elvalue
+  end.
+Ltac crush_eval_lvalue :=
+  cbn;
+  lazymatch goal with
+  | [ |- eval_lvalue _ _ _ _ (Evar _ _) _ _ ] =>
+      solve [ apply eval_Evar_local; reflexivity | apply eval_Evar_global; [ reflexivity | eassumption ] ]
+  | _ => constructor
+  end.
+Ltac crush_deref :=
+  cbn;
+  lazymatch goal with
+  | [ |- deref_loc (Tarray _ _ _) _ _ _ _] => eapply deref_loc_reference; reflexivity
+  | [ |- deref_loc (Tfunction _ _ _) _ _ _ _] => eapply deref_loc_reference; reflexivity
+  | [ |- deref_loc (Tint _ _ _) _ _ _ _] => eapply deref_loc_value; [ reflexivity | ]
+  end.
+
+Ltac crush_expr :=
+  repeat (cbn;
+    match goal with
+    | [ |- eval_expr _ _ _ _ _ _ _ ] => crush_eval_expr
+    | [ |- eval_lvalue _ _ _ _ _ _ _ _ ] => crush_eval_lvalue
+    | [ |- eval_exprlist _ _ _ _ _ _ _ _ ] => econstructor
+    | [ |- deref_loc _ _ _ _ _ ] => crush_deref
+    | [ |- Cop.sem_binary_operation _ _ _ _ _ _ _ = Some _] => try reflexivity
+    | [ |- Cop.sem_cast _ ?ty ?ty _ = Some _ ] => apply Cop.cast_val_casted; eauto
+    | [ |- assign_loc _ (Tint _ _ _) _ _ _ _ _ ] => eapply assign_loc_value; [ reflexivity | ]
+    | _ => try solve [ easy | eassumption ]
+    end).
+
+Ltac prove_norepet H :=
+  match type of H with
+  | False => inversion H
+  | (?a = ?b) \/ _ =>
+      destruct H as [H|H]; [inversion H|prove_norepet H]
+  end.
+
+Ltac solve_list_norepet :=
+  simpl;
+  match goal with
+  | |- list_norepet nil =>  apply list_norepet_nil
+  | |- list_norepet (?x :: ?l) =>
+      apply list_norepet_cons;
+      [simpl; let H := fresh "H" in intro H; prove_norepet H |solve_list_norepet]
+  end.
+Ltac destruct_or H :=
+  match type of H with
+  | _ \/ _ => destruct H as [H|H]; [ |destruct_or H]
+  | _ => idtac
+  end.
+
+Ltac solve_list_disjoint :=
+  simpl; unfold list_disjoint; simpl; red;
+  let x := fresh "x" in
+  let y := fresh "y" in
+  let Lx := fresh "Lx" in
+  let Ly := fresh "Ly" in
+  let xyEq := fresh "xyEq" in
+  intros x y Lx Ly xyEq; try rewrite xyEq in *; clear xyEq;
+  destruct_or Lx; destruct_or Ly; subst; try solve [inversion Lx]; try solve [inversion Ly].
+
+Ltac crush_step := cbn;
+  match goal with
+  | [ |- Step _ (Callstate _ _ _ _, _) _ _ ] =>
+      eapply step_internal_function;
+      [ eauto | constructor; cbn;
+        [ solve_list_norepet
+        | solve_list_norepet
+        | solve_list_disjoint
+        | repeat (econstructor; simpl; auto)
+        | reflexivity | eauto ] ]
+  | [ |- Step _ (State _ (Ssequence _ _) _ _ _ _, _) _ _ ] => apply step_seq
+  | [ |- Step _ (State _ (Sset _ _) _ _ _ _, _) _ _ ] => apply step_set
+  | [ |- Step _ (State _ (Scall _ _ _) _ _ _ _, _) _ _ ] => eapply step_call
+  | [ |- Step _ (Returnstate _ _ _, _) _ _ ] => eapply step_returnstate
+  | [ |- Step _ (State _ Sskip (Kseq _ _) _ _ _, _) _ _ ] => apply step_skip_seq
+  | [ |- Step _ (State _ (Sassign _ _) _ _ _ _, _) _ _ ] => eapply step_assign
+  | [ |- Step _ (State _ (Sreturn None) _ _ _ _, _) _ _ ] => eapply step_return_0
+  | [ |- Step _ (State _ (Sreturn (Some _)) _ _ _ _, _) _ _ ] => eapply step_return_1
+  | [ |- Step _ (State _ ?s _ _ _ _, _) _ _ ] => is_const s; unfold s; crush_step
+  end.
+
+Ltac lts_step := eapply star_left with (t1 := E0) (t2 := E0); [ | | reflexivity ].
+
+Ltac crush_star :=
+  match goal with
+  | [ |- Star _ (Returnstate _ Kstop _) _ _ ] => eapply star_refl
+  | _ => lts_step; [ crush_step; crush_expr | cbn; try crush_star ]
+  end.
+
+Opaque clightp1.
+Opaque PTree.set.
+Opaque Nat.modulo.
+
+Require Import Lia.
+
+Lemma cnt_inc_simp c i:
+  Z.of_nat c = Int.intval i -> (c < N)%nat ->
+  Z.of_nat (S c mod N) = Int.intval (Int.modu (Int.add i (Int.repr 1)) (Int.repr Nz)).
+Proof.
+  intros H1 H2. unfold Int.add, Int.modu.
+  apply inj_le in H2. rewrite Nat2Z.inj_succ in H2.
+  rewrite H1 in H2.
+  repeat rewrite Int.unsigned_repr.
+  all: unfold Nz in *; cbn -[Z.mul] in *; unfold Int.unsigned; try lia.
+  - unfold Int.unsigned. rewrite <- H1.
+    rewrite mod_Zmod.
+    + f_equal. rewrite Nat2Z.inj_succ. reflexivity.
+    + unfold N. lia.
+  - unfold Int.unsigned. rewrite <- H1.
+    exploit (Z.mod_pos_bound (Z.of_nat c + 1) (Z.of_nat N)); unfold N; lia.
+Qed.
+
+Lemma cop_sem_mod m i j:
+  j <> Int.zero -> Cop.sem_mod (Vint i) tint (Vint j) tint m = Some (Vint (Int.modu i j)).
+Proof.
+  intros Hj. unfold Cop.sem_mod.
+  unfold Cop.sem_binarith. cbn.
+  unfold Cop.sem_cast. cbn.
+  destruct Archi.ptr64. cbn.
+  rewrite Int.eq_false; eauto.
+  rewrite Int.eq_false; eauto.
+Qed.
+
+Hint Constructors rb_func_rel.
+Opaque clightp2.
+
+Lemma rb_correct2: forward_simulation 1 rb_cc rb_spec (clightp2 rb_program).
+Proof.
+  constructor. econstructor. reflexivity. firstorder.
+  intros. instantiate (1 := fun _ _ _ => _). cbn beta.
+  destruct H. set (ms := fun s1 s2 => rb_ms se1 s1 s2).
+  eapply forward_simulation_plus with (match_states := ms).
+  - intros [q1 rs1] [q2 pe] s1 Hq Hs. inv Hq. cbn in *. subst. inv Hs.
+    (* TODO: cleanup by ltac *)
+    + eexists (_, _). split.
+      * econstructor; eauto.
+        eapply genv_funct_symbol; eauto. reflexivity.
+        reflexivity. constructor.
+      * econstructor; eauto.
+        eapply genv_funct_symbol; eauto.
+    + eexists (_, _). split.
+      * econstructor; eauto.
+        eapply genv_funct_symbol; eauto. reflexivity.
+        reflexivity. constructor.
+      * econstructor; eauto.
+        eapply genv_funct_symbol; eauto.
+    + eexists (_, _). split.
+      * econstructor; eauto.
+        eapply genv_funct_symbol; eauto. reflexivity.
+        reflexivity. repeat constructor; eauto.
+      * econstructor; eauto.
+        eapply genv_funct_symbol; eauto.
+    + eexists (_, _). split.
+      * econstructor; eauto.
+        eapply genv_funct_symbol; eauto. reflexivity.
+        reflexivity. repeat constructor; eauto.
+      * econstructor; eauto.
+        eapply genv_funct_symbol; eauto.
+  - intros. cbn in *. eprod_crush. inv H1. inv H.
+    eexists (_, _). split; constructor; cbn; eauto.
+  - intros. inv H1.
+  - intros * HS [s2 pe] HM. inv HS; inv HM.
+    (* inc1 *)
+    + inv HPE. inv RC1. inv HFUN. eexists (_, _). split.
+      * eapply plus_left. crush_step.
+        lts_step. crush_step.
+        lts_step. crush_step.
+        lts_step. crush_step.
+        lts_step. crush_step.
+        { eapply eval_Eloc; eauto.
+          repeat econstructor; eauto.
+          repeat econstructor; eauto. }
+        lts_step. crush_step.
+        lts_step.
+        {
+          eapply step_update; eauto.
+          + econstructor; eauto.
+          + crush_expr.
+            * eapply eval_Eloc; eauto.
+              repeat econstructor. eauto.
+              repeat econstructor. eauto.
+            * reflexivity.
+          + econstructor; eauto; try easy.
+            constructor; eauto.
+            constructor. reflexivity.
+          + constructor. reflexivity.
+        }
+        lts_step. crush_step.
+        lts_step.
+        {
+          eapply step_update; eauto.
+          + econstructor; eauto. rewrite PTree.gss. reflexivity.
+          + crush_expr.
+            * eapply eval_Eloc; eauto.
+              econstructor; eauto.
+              rewrite PTree.gss. reflexivity.
+              econstructor; eauto.
+              rewrite PTree.gss. reflexivity.
+              constructor.
+            * reflexivity.
+          + econstructor; eauto; try easy.
+            rewrite PTree.gss. reflexivity.
+            constructor; eauto.
+            constructor. reflexivity.
+          + constructor. reflexivity.
+        }
+        lts_step. crush_step.
+        lts_step. crush_step; crush_expr. now constructor.
+        apply star_refl. reflexivity.
+      * cbn. rewrite HI.
+        replace (Int.repr (Int.intval i)) with i
+          by now rewrite Int.repr_unsigned.
+        econstructor; eauto. econstructor; eauto.
+        -- rewrite PTree.gso. rewrite PTree.gso. eauto.
+           all: unfold arr_id, cnt1_id; lia.
+        -- rewrite PTree.gss. reflexivity.
+        -- rewrite PTree.gso. rewrite PTree.gso. eauto.
+           all: unfold cnt2_id, cnt1_id; lia.
+        -- constructor. apply cnt_inc_simp; eauto.
+        -- apply Nat.mod_upper_bound. lia.
+    (* inc2 *)
+    + admit.
+    (* get *)
+    + inv HPE. inv HFUN.
+      edestruct RA as (v & HV1 & HV2). apply H1.
+      eexists (_, _). split.
+      * eapply plus_left. crush_step.
+        lts_step. crush_step; crush_expr.
+        {
+          eapply eval_Eloc; eauto.
+          - econstructor; eauto.
+            + reflexivity.
+            + econstructor; eauto.
+            + crush_expr.
+            + admit.
+          - econstructor; eauto.
+            econstructor; eauto.
+            admit.
+            cbn.
+            rewrite Int.unsigned_repr.
+            rewrite HV1. econstructor.
+            admit.
+        }
+        admit.
+        apply star_refl. reflexivity.
+      * subst. constructor; eauto.
+        econstructor; eauto.
+  (* set *)
+    + admit.
+  - apply well_founded_ltof.
+Admitted.
+
+Lemma rb_correct:
+  E.forward_simulation (&1) (&1) rb_espec (eclightp rb_program).
+Proof.
+  eapply encap_fsim_lcomp_sk; eauto. instantiate (1 := &rb_cc).
+  - apply rb_correct1.
+  - apply encap_fsim_embed. apply rb_correct2.
+  - cbn. apply ClightPComp.id_skel_least.
+  - cbn. apply Linking.linkorder_refl.
+Qed.
 
 (** ------------------------------------------------------------------------- *)
 (** Bounded Queue Spec *)
@@ -476,10 +822,10 @@ Section RB_LTS.
     {|
       Smallstep.genvtype := genv;
       Smallstep.step ge := bq_step;
-      Smallstep.initial_state := bq_initial_state;
+      Smallstep.initial_state q := bq_initial_state q;
       Smallstep.at_external := bq_at_external;
       Smallstep.after_external := bq_after_external;
-      Smallstep.final_state := bq_final_state;
+      Smallstep.final_state s r := bq_final_state s r;
       Smallstep.globalenv := ge;
     |}.
 
@@ -492,10 +838,46 @@ Definition bq_spec: semantics li_c li_c :=
     footprint := AST.footprint_of_program bq_program;
   |}.
 
+Program Definition bq_cc: callconv li_c (li_c@penv).
+Admitted.
+
+Lemma bq_correct1:
+  E.forward_simulation (&bq_cc) (&1) (semantics_embed 1)
+    (@encap_prim penv (penv_pset (ClightPComp.vars_of_program bq_program))).
+Proof.
+Admitted.
+
+Lemma bq_correct2: forward_simulation 1 bq_cc bq_spec (clightp2 bq_program).
+Proof.
+Admitted.
+
 Definition bq_espec: li_c +-> li_c := semantics_embed bq_spec.
 
+
 Lemma bq_correct: E.forward_simulation (&1) (&1) bq_espec (eclightp bq_program).
+Proof.
+  rewrite ccref_left_unit1 at 2.
+  rewrite <- ccref_left_unit2 at 1.
+  eapply encap_fsim_vcomp.
+  instantiate (1 := comp_esem' (semantics_embed 1%lts) bq_espec (skel bq_spec)).
+  (* TODO: we need a lemma here *)
+  - rewrite ccref_left_unit1 at 2.
+    rewrite <- ccref_left_unit2 at 1.
+    eapply encap_fsim_vcomp; eauto.
+    instantiate (1 := semantics_embed _).
+    + apply encap_fsim_embed_cat.
+      apply CAT.left_unit_1.
+    + unfold left_comp_id.
+      (* symmetric version of encap_comp_embed *)
+      admit.
+  - eapply encap_fsim_lcomp_sk. instantiate (1 := &bq_cc).
+    + apply bq_correct1.
+    + apply encap_fsim_embed.
+      apply bq_correct2.
+    + apply ClightPComp.id_skel_least.
+    + apply Linking.linkorder_refl.
 Admitted.
+
 
 (** ------------------------------------------------------------------------- *)
 (** Abstract Ring Buffer Spec *)
@@ -572,24 +954,326 @@ Section REFINE.
                          \/ footprint_of_program rb_program i;
     |}.
 
-  Instance bq_state_pset : PSet bq_state. Admitted.
+  Instance bq_state_pset : PSet bq_state :=
+    { pset_init _ := nil; }.
 
   Definition abs_bq_espec : li_c +-> li_c :=
     comp_esem'
       (encap_prim bq_state)
       (semantics_embed abs_bq_spec)
-      (skel bq_spec).
+      rb_bq_skel.
+
+  Open Scope nat_scope.
+
+  Fixpoint slice (f : nat -> Values.val) (i : nat) (n : nat) : list Values.val :=
+    match n with
+    | O => nil
+    | S n' => f i :: slice f (S i mod N) n'
+    end.
+
+  Inductive rb_bq : bq_state -> rb_state -> Prop :=
+    bq_rb_intro f c1 c2 n q :
+      c1 < N ->
+      n <= N ->
+      q = slice f c1 n ->
+      c2 = (c1 + n) mod N ->
+      (forall i, Cop.val_casted (f i) tint) ->
+      rb_bq q (f, c1, c2).
+
+  Import Relators.
+
+  Program Definition abs_bq_cc: callconv (li_c@bq_state) (li_c@rb_state) :=
+    {|
+      ccworld := unit;
+      match_senv _ := eq;
+      match_query _ := (eq * rb_bq)%rel;
+      match_reply _ := (eq * rb_bq)%rel;
+    |}.
+  Next Obligation. reflexivity. Qed.
+  Next Obligation. inv H0. cbn in *. subst. reflexivity. Qed.
+  Next Obligation. inv H. cbn in *. subst. reflexivity. Qed.
+
+  Definition bq_rb_spec :=
+    CategoricalComp.comp_semantics' (bq_spec @ rb_state) rb_spec rb_bq_skel.
+  Definition bq_rb_espec :=
+    comp_esem' (encap_prim rb_state) (semantics_embed bq_rb_spec) rb_bq_skel.
+
+  Inductive bq_abs_ms se: bq_abs_state -> comp_state (bq_spec @ rb_state) rb_spec -> Prop :=
+  | bq_abs_ms_enq:
+    forall m v rbst bqst
+      (HR: rb_bq bqst rbst)
+      (HB: Ple (Genv.genv_next se) (Mem.nextblock m))
+      (HV: Cop.val_casted v tint),
+      bq_abs_ms se  (bq_abs_init enq bqst [v] m)
+        (st1 (bq_spec @ rb_state) _ (bq_init enq [v] m, rbst))
+  | bq_abs_ms_deq:
+    forall m rbst bqst
+      (HR: rb_bq bqst rbst)
+      (HB: Ple (Genv.genv_next se) (Mem.nextblock m)),
+      bq_abs_ms se (bq_abs_init deq bqst nil m)
+        (st1 (bq_spec @ rb_state) _ (bq_init deq nil m, rbst))
+  | bq_abs_ms_final:
+    forall rv m bqst rbst
+      (HR: rb_bq bqst rbst),
+      bq_abs_ms se (bq_abs_final bqst rv m)
+        (st1 (bq_spec @ rb_state) _ (bq_final rv m, rbst)).
+
+  Lemma bq_refine1:
+    E.forward_simulation (&abs_bq_cc) (&1)
+      (encap_prim bq_state) (encap_prim rb_state).
+  Proof.
+  Admitted.
+
+  Lemma rb_bq_c2:
+    forall q f c1 c2,
+      rb_bq q (f, c1, c2) -> c2 < N.
+  Proof.
+    intros. inv H. apply Nat.mod_upper_bound. unfold N. omega.
+  Qed.
+
+  Lemma refine_correct1:
+    forall v vs f c1 c2,
+      rb_bq (v :: vs) (f, c1, c2) ->
+      v = f c1 /\ rb_bq vs (f, S c1 mod N, c2).
+  Admitted.
+
+  Lemma slice_length f c1 n :
+    List.length (slice f c1 n) = n.
+  Proof.
+  Admitted.
+
+  Lemma mod_minus:
+    forall a, N <= a < N * 2 -> a mod N = a - N.
+  Proof.
+  Admitted.
+
+  Lemma mod_add_not_same a b:
+    a < N -> b < N -> b <> 0 -> (a + b) mod N <> a.
+  Proof.
+  Admitted.
+
+  Lemma refine_correct2:
+    forall v vs f c1 c2,
+      List.length vs < N ->
+      Cop.val_casted v tint ->
+      rb_bq vs (f, c1, c2) ->
+      rb_bq (vs++[v]) (fun j : nat => if Nat.eq_dec c2 j then v else f j, c1, S c2 mod N).
+  Proof.
+  Admitted.
+
+  Import Ptrofs.
+  Lemma inc2_block se:
+    Genv.valid_for (clightp_erase_program bq_program) se ->
+    exists b, Genv.find_symbol (globalenv se bq_program) inc2_id = Some b /\
+           Genv.find_funct (globalenv se bq_program) (Vptr b zero) = Some inc2_ext.
+  Proof.
+  (*   intros Hse. eapply Genv.find_def_symbol with (id := inc2_id) in Hse . *)
+  (*   edestruct (proj1 Hse) as (b & Hb1 & Hb2). reflexivity. *)
+  (*   exists b. split; eauto. eapply genv_funct_symbol; eauto. *)
+  (* Qed. *)
+  Admitted.
+
+  Lemma set_block se:
+    Genv.valid_for (clightp_erase_program bq_program) se ->
+    exists b, Genv.find_symbol (globalenv se bq_program) set_id = Some b /\
+           Genv.find_funct (globalenv se bq_program) (Vptr b zero) = Some set_ext.
+  Proof.
+  (*   intros Hse. eapply Genv.find_def_symbol with (id := set_id) in Hse . *)
+  (*   edestruct (proj1 Hse) as (b & Hb1 & Hb2). reflexivity. *)
+  (*   exists b. split; eauto. eapply genv_funct_symbol; eauto. *)
+  (* Qed. *)
+  Admitted.
+  Lemma inc1_block se:
+    Genv.valid_for (clightp_erase_program bq_program) se ->
+    exists b, Genv.find_symbol (globalenv se bq_program) inc1_id = Some b /\
+           Genv.find_funct (globalenv se bq_program) (Vptr b zero) = Some inc1_ext.
+  Proof.
+  Admitted.
+  (*   intros Hse. eapply Genv.find_def_symbol with (id := inc1_id) in Hse . *)
+  (*   edestruct (proj1 Hse) as (b & Hb1 & Hb2). reflexivity. *)
+  (*   exists b. split; eauto. eapply genv_funct_symbol; eauto. *)
+  (* Qed. *)
+
+  Lemma get_block se:
+    Genv.valid_for (clightp_erase_program bq_program) se ->
+    exists b, Genv.find_symbol (globalenv se bq_program) get_id = Some b /\
+           Genv.find_funct (globalenv se bq_program) (Vptr b zero) = Some get_ext.
+  Proof.
+  Admitted.
+  (*   intros Hse. eapply Genv.find_def_symbol with (id := get_id) in Hse . *)
+  (*   edestruct (proj1 Hse) as (b & Hb1 & Hb2). reflexivity. *)
+  (*   exists b. split; eauto. eapply genv_funct_symbol; eauto. *)
+  (* Qed. *)
+  (* Opaque Genv.find_funct semantics2. *)
+
+  Opaque clightp2.
+  Import CategoricalComp.
+
+  Lemma bq_refine2:
+    forward_simulation 1 abs_bq_cc abs_bq_spec bq_rb_spec.
+  Proof.
+    constructor. econstructor. reflexivity. firstorder.
+    intros. instantiate (1 := fun _ _ _ => _). cbn beta.
+    destruct H. destruct wB.
+    eapply forward_simulation_plus with (match_states := bq_abs_ms se1).
+    - intros. cbn in *. eprod_crush. inv H. cbn in *. inv H1.
+      + eexists. split.
+        * econstructor.  instantiate (1 := (_, _)).
+          constructor; cbn. econstructor; eauto. reflexivity.
+        * econstructor; eauto.
+      + eexists. split.
+        * econstructor.  instantiate (1 := (_, _)).
+          constructor; cbn. econstructor; eauto. reflexivity.
+        * econstructor; eauto.
+    - intros. inv H; inv H1.
+      eexists (_, _). split; repeat constructor. eauto.
+    - intros. inv H1.
+    - intros. inv H1; inv H.
+      (* enq *)
+      + exploit (inc2_block se1). cbn in *.
+        eapply Genv.valid_for_linkorder; eauto.
+        admit.
+        (* apply Linking.linkorder_erase. apply bq_linkorder. *)
+        intros (b1 & A & B).
+        exploit (set_block se1).
+        eapply Genv.valid_for_linkorder; eauto.
+        admit.
+        (* apply linkorder_erase. apply bq_linkorder. *)
+        intros (b2 & C & D).
+        destruct rbst as [[f c1] c2].
+        eexists. split.
+        * eapply plus_left. cbn. constructor.
+          { instantiate (1 := (_, _)). constructor; eauto. constructor. }
+          lts_step.
+          {
+            eapply step_push.
+            - instantiate (1 := (_, _)).  constructor; cbn.
+              econstructor; eauto. eauto.
+            - eapply initial_state_inc2; eauto.
+          }
+          lts_step.
+          { apply step2. constructor. reflexivity. }
+          lts_step.
+          {
+            eapply step_pop.
+            - constructor.
+            - instantiate (1 := (_, _)). constructor; cbn.
+              constructor. constructor. cbn. reflexivity. reflexivity.
+          }
+          lts_step.
+          { apply step1. instantiate (1 := (_, _)).
+            constructor; eauto. constructor. }
+          lts_step.
+          {
+            eapply step_push.
+            - instantiate (1 := (_, _)).  constructor; cbn.
+              econstructor; eauto. eauto.
+            - econstructor; eauto. constructor. reflexivity.
+          }
+          lts_step.
+          { eapply step2. constructor; eauto. eapply rb_bq_c2; eauto. }
+          lts_step.
+          {
+            eapply step_pop.
+            - constructor.
+            - instantiate (1 := (_, _)). constructor; cbn.
+              constructor. reflexivity.
+          }
+          lts_step.
+          { eapply step1. instantiate (1 := (_, _)). repeat constructor. }
+          apply star_refl. reflexivity.
+        * constructor. now apply refine_correct2.
+      (* deq *)
+      + exploit (inc1_block se1).
+        eapply Genv.valid_for_linkorder; eauto.
+        (* apply linkorder_erase. apply bq_linkorder. *)
+        admit.
+        intros (b1 & A & B).
+        exploit (get_block se1).
+        eapply Genv.valid_for_linkorder; eauto.
+        (* apply linkorder_erase. apply bq_linkorder. *)
+        admit.
+        intros (b2 & C & D).
+        destruct rbst as [[f c1] c2].
+        eexists. split.
+        * eapply plus_left. cbn. constructor.
+          { instantiate (1 := (_, _)). constructor; eauto. constructor. }
+          lts_step.
+          {
+            eapply step_push.
+            - instantiate (1 := (_, _)).  constructor; cbn.
+              econstructor; eauto. eauto.
+            - eapply initial_state_inc1; eauto.
+          }
+          lts_step.
+          { eapply step2. constructor. reflexivity. }
+          lts_step.
+          {
+            eapply step_pop.
+            - constructor.
+            - instantiate (1 := (_, _)). constructor; cbn.
+              constructor. constructor. cbn. reflexivity. reflexivity.
+          }
+          lts_step.
+          { apply step1. instantiate (1 := (_, _)).
+            constructor; eauto. constructor. }
+          lts_step.
+          {
+            eapply step_push.
+            - instantiate (1 := (_, _)).  constructor; cbn.
+              econstructor; eauto. eauto.
+            - econstructor; eauto.
+              constructor. reflexivity.
+          }
+          lts_step.
+          { eapply step2. constructor. reflexivity. inv HR; eauto. }
+          lts_step.
+          {
+            eapply step_pop.
+            - constructor.
+            - instantiate (1 := (_, _)). constructor; cbn.
+              constructor. inv HR. apply H8. reflexivity.
+          }
+          lts_step.
+          { eapply step1. instantiate (1 := (_, _)). repeat constructor. }
+          apply star_refl. reflexivity.
+        * eapply refine_correct1 in HR as [X Y]. subst.
+          constructor. auto.
+    - apply well_founded_ltof.
+  Admitted.
 
   Lemma bq_refine:
     E.forward_simulation
-      (&1) (&1) bq_espec
-      (comp_esem' bq_espec rb_espec rb_bq_skel).
+      (&1) (&1) abs_bq_espec (comp_esem' bq_espec rb_espec rb_bq_skel).
+  Proof.
+    rewrite ccref_left_unit1 at 2.
+    rewrite <- ccref_left_unit2 at 1.
+    eapply encap_fsim_vcomp.
+    instantiate (1 := bq_rb_espec).
+    - eapply encap_fsim_lcomp_sk.
+      instantiate (1 := &abs_bq_cc).
+      + apply bq_refine1.
+      + apply encap_fsim_embed.
+        apply bq_refine2.
+      + apply ClightPComp.id_skel_least.
+      + apply Linking.linkorder_refl.
+    - unfold bq_rb_espec.
   Admitted.
 
   Lemma rb_bq_correct:
     E.forward_simulation
       (&1) (&1) abs_bq_espec
       (comp_esem' (eclightp bq_program) (eclightp rb_program) rb_bq_skel).
+  Proof.
+    rewrite ccref_left_unit1 at 2.
+    rewrite <- ccref_left_unit2 at 1.
+    eapply encap_fsim_vcomp.
+    - apply bq_refine.
+    - eapply encap_fsim_lcomp_sk.
+      + apply bq_correct.
+      + apply rb_correct.
+      + admit.
+      + admit.
   Admitted.
 
 End REFINE.
